ChoiceTyping/theories/Auxiliary.v
@@ -7,16 +7,30 @@ From ChoiceTyping Require Export WellFormed.
 
 (** ** Semantic subtyping and context restriction *)
 
-Definition sub_type (Γ : ctx) (τ1 τ2 : choice_ty) : Prop :=
-  wf_choice_ty Γ τ1 ∧
-  wf_choice_ty Γ τ2 ∧
+Definition sub_type_under (Σ : gmap atom ty) (Γ : ctx) (τ1 τ2 : choice_ty) : Prop :=
+  wf_choice_ty_under Σ Γ τ1 ∧
+  wf_choice_ty_under Σ Γ τ2 ∧
   erase_ty τ1 = erase_ty τ2 ∧
-  ∀ e, fv_tm e ⊆ ctx_dom Γ →
-    ⟦Γ⟧ ⊫ FImpl (denot_ty_in_ctx Γ τ1 e) (denot_ty_in_ctx Γ τ2 e).
+  ∀ e, fv_tm e ⊆ dom Σ ∪ ctx_dom Γ →
+    denot_ctx_in_env Σ Γ ⊫
+      FImpl (denot_ty_in_ctx_under Σ Γ τ1 e)
+            (denot_ty_in_ctx_under Σ Γ τ2 e).
+
+Definition sub_type (Γ : ctx) (τ1 τ2 : choice_ty) : Prop :=
+  sub_type_under ∅ Γ τ1 τ2.
+
+Definition ctx_sub_under
+    (Σ : gmap atom ty) (X : aset) (Γ1 Γ2 : ctx) : Prop :=
+  wf_ctx_under Σ Γ1 ∧
+  wf_ctx_under Σ Γ2 ∧
+  ty_env_agree_on X (erase_ctx_under Σ Γ1) (erase_ctx_under Σ Γ2) ∧
+  ∀ r, r ⊨ denot_ctx_in_env Σ Γ1 →
+       res_restrict r X ⊨ denot_ctx_in_env Σ Γ2.
 
 Definition ctx_sub (X : aset) (Γ1 Γ2 : ctx) : Prop :=
   wf_ctx Γ1 ∧
   wf_ctx Γ2 ∧
+  ty_env_agree_on X (erase_ctx Γ1) (erase_ctx Γ2) ∧
   ∀ r, r ⊨ ⟦Γ1⟧ → res_restrict r X ⊨ ⟦Γ2⟧.
 
 Definition ctx_to_over (Γ Γ' : ctx) : Prop :=
@@ -51,6 +65,14 @@ Lemma ctx_sub_wf_r X Γ1 Γ2 :
   wf_ctx Γ2.
 Proof. intros [_ [Hwf _]]. exact Hwf. Qed.
 
+Lemma ctx_sub_env_agree X Γ1 Γ2 :
+  ctx_sub X Γ1 Γ2 →
+  ty_env_agree_on X (erase_ctx Γ1) (erase_ctx Γ2).
+Proof.
+  intros [_ [_ [Hagree _]]].
+  exact Hagree.
+Qed.
+
 Lemma ctx_to_over_wf_l Γ Γ' :
   ctx_to_over Γ Γ' →
   wf_ctx Γ.
@@ -69,7 +91,7 @@ Proof.
   split; [exact Hwf |]. split; [exact Hwf |]. split; [reflexivity |].
   intros e Hfv m HΓ.
   apply res_models_impl_refl.
-  eapply denot_ty_scoped_from_ctx; eauto.
+  eapply denot_ty_scoped_from_ctx_under; eauto.
 Qed.
 
 Lemma ctx_sub_refl Γ :
@@ -77,7 +99,9 @@ Lemma ctx_sub_refl Γ :
   ctx_sub (ctx_stale Γ) Γ Γ.
 Proof.
   intros Hwf.
-  split; [exact Hwf |]. split; [exact Hwf |].
+  split; [exact Hwf |]. split; [exact Hwf |]. split.
+  - intros x Hx. reflexivity.
+  -
   intros r Hr.
   apply denot_ctx_restrict_stale. exact Hr.
 Qed.
